base case

theories/vir/mcfg_contextual.v
@@ -8,16 +8,41 @@ From velliris.vir Require Import
 From Vellvm Require Import Syntax.DynamicTypes Handlers Syntax.LLVMAst
   Semantics.InterpretationStack.
 
-From ITree Require Import ITree Recursion.
+From Equations Require Import Equations.
+
+From ITree Require Import ITree Recursion Eq.Eqit.
 From Equations Require Import Equations.
 
 Import LLVMEvents.
 
 Set Default Proof Using "Type*".
 
+Opaque mrec.
+
+(* -------------------------------------------------------------------------- *)
+
+(* ITree-related tactics *)
+Ltac obs_hyp :=
+  match goal with
+  | [ H : {| _observe := observe _ |} = _ |- _] =>
+      let Hobs := fresh "Hobs" in
+      inversion H as [ Hobs ]; clear H
+  end.
+
+(* Turn an [observe] hypothesis to an ITree equivalence. *)
+Ltac simpobs_eqit :=
+  obs_hyp;
+  match goal with
+  | [ H : observe _ = _ |- _] =>
+      symmetry in H; apply Eqit.simpobs in H
+  end.
+
 Section mcfg_contextual.
 
   Context `(sheapGS Σ, checkedoutGS Σ, heapbijGS Σ).
+
+  Definition args_rel :=
+    fun args_t args_s => ([∗ list] x;y ∈ args_t ;args_s, uval_rel x y)%I.
 
   (* Invariant for frame-related resources across a single function call that
      is satisfied by the fundamental theorem *)
@@ -29,60 +54,71 @@ Section mcfg_contextual.
   Definition context_rel
       (f : ∀ T : Type, CallE T → L0'expr T)
       (g : ∀ T : Type, CallE T → L0'expr T) :=
-    (□ (∀ fn1 fn2 dt1 dt2 args1 args2 C,
+    (∀ fn1 fn2 dt1 dt2 args1 args2 C,
           let call1 := ExternalCall dt1 fn1 args1 nil in
           let call2 := ExternalCall dt2 fn2 args2 nil in
           call_ev call1 call2 C -∗
           ⟅ f _ (Call dt1 fn1 args1 nil) ⟆ ⪯
           ⟅ g _ (Call dt2 fn2 args2 nil) ⟆
-          [[ (fun v1 v2 => call_ans call1 v1 call2 v2 C) ⤉ ]]) )%I.
+          [[ (fun v1 v2 => call_ans call1 v1 call2 v2 C) ⤉ ]])%I.
 
   Notation st_expr_rel' R1 R2 :=
     (@st_exprO' vir_lang R1 -d> @st_exprO' vir_lang R2 -d> iPropI Σ).
 
+  Definition contains_base {T} Φ :=
+    (∀ x y : st_exprO' T, base x y ∗ Φ x y ∗-∗ Φ x y : iProp Σ)%I.
+
   (* Auxiliary definitions for [Proper_interp_mrec] *)
   (* Because [sim_expr] includes stateful interpretation, showing properness result
     for [interp_mrec] amounts to proving a simulation *)
-  Local Definition interp_mrec_pred :=
+  Local Definition mrec_pred :=
     fun (Φ:st_expr_rel' _ _) (e_t:st_expr' vir_lang _) (e_s:st_expr' vir_lang _) =>
       (∃ f g t dv args attr σ_t σ_s,
-          ⌜e_t = observe (⟦ interp_mrec f (f uvalue (Call t dv args attr)) ⟧ σ_t)⌝ ∗
-          ⌜e_s = observe (⟦ interp_mrec g (g uvalue (Call t dv args attr)) ⟧ σ_s)⌝ ∗
-          context_rel f g ∗
+          ⌜e_t = observe (⟦ mrec f (Call t dv args attr) ⟧ σ_t)⌝ ∗
+          ⌜e_s = observe (⟦ mrec g (Call t dv args attr) ⟧ σ_s)⌝ ∗
+          (* Function is called on related addresses and arguments *)
+          dval_rel dv dv ∗
+          args_rel args args ∗
+          (* Postcondition contains [base] predicate*)
+          □ contains_base Φ ∗
+          (* Contexts are related *)
+          □ context_rel f g ∗
           sim_coindF Φ
-              (observe (⟦ ⟅ (f uvalue (Call t dv args attr)) ⟆ ⟧ σ_t))
-              (observe (⟦ ⟅ (g uvalue (Call t dv args attr)) ⟆ ⟧ σ_s)))%I.
+              (observe (⟦ ⟅ f uvalue (Call t dv args attr) ⟆ ⟧ σ_t))
+              (observe (⟦ ⟅ g uvalue (Call t dv args attr) ⟆ ⟧ σ_s)))%I.
 
-  Local Definition interp_mrec_rec :=
+  Local Definition mrec_rec :=
     fun (Φ:st_expr_rel' _ _) (e_t:st_expr' vir_lang _) (e_s:st_expr' vir_lang _) =>
       ((∃ f g t dv args attr σ_t σ_s,
-          ⌜e_t = observe (⟦ interp_mrec f (f uvalue (Call t dv args attr)) ⟧ σ_t)⌝ ∗
-          ⌜e_s = observe (⟦ interp_mrec g (g uvalue (Call t dv args attr)) ⟧ σ_s)⌝ ∗
-         context_rel f g ∗
+          ⌜e_t = observe (⟦ mrec f (Call t dv args attr) ⟧ σ_t)⌝ ∗
+          ⌜e_s = observe (⟦ mrec g (Call t dv args attr) ⟧ σ_s)⌝ ∗
+          dval_rel dv dv ∗ args_rel args args ∗
+          □ contains_base Φ ∗
+          □ context_rel f g ∗
          sim_coindF Φ
-          (observe (⟦ ⟅ (f uvalue (Call t dv args attr)) ⟆ ⟧ σ_t))
-          (observe (⟦ ⟅ (g uvalue (Call t dv args attr)) ⟆ ⟧ σ_s)))
+          (observe (⟦ ⟅ f uvalue (Call t dv args attr) ⟆ ⟧ σ_t))
+          (observe (⟦ ⟅ g uvalue (Call t dv args attr) ⟆ ⟧ σ_s)))
         ∨ sim_coindF Φ e_t e_s)%I.
 
-  Local Instance interp_mrec_pred_ne:
-    NonExpansive (interp_mrec_pred: st_expr_rel' _ _ -d> st_expr_rel' _ _).
+  Local Instance mrec_pred_ne:
+    NonExpansive (mrec_pred: st_expr_rel' _ _ -d> st_expr_rel' _ _).
   Proof.
-    intros x y *. solve_proper_prepare. do 18 f_equiv; try solve_proper.
+    intros x y *. solve_proper_prepare. do 22 f_equiv; try solve_proper.
   Qed.
 
-  Local Instance interp_mrec_rec_ne:
-    NonExpansive (interp_mrec_rec: st_expr_rel' _ _ -d> st_expr_rel' _ _).
+  Local Instance mrec_rec_ne:
+    NonExpansive (mrec_rec: st_expr_rel' _ _ -d> st_expr_rel' _ _).
   Proof.
-    intros x y *. solve_proper_prepare. repeat f_equiv; try solve_proper.
-  Qed.
-
-  From Equations Require Import Equations.
-
-  Definition args_rel :=
-    fun args_t args_s => ([∗ list] x;y ∈ args_t ;args_s, uval_rel x y)%I.
+    intros x y *. solve_proper_prepare.
+  Admitted.
 
   (* -------------------------------------------------------------------------- *)
+  (* Local notations to make life "easier".. *)
+  Local Notation sim_mrec_ind := (sim_expr_inner mrec_rec (sim_indF mrec_rec)).
+  Local Notation "o⟦ e ⟧ σ" := (observe (⟦ e ⟧ σ)) (at level 12).
+  (* -------------------------------------------------------------------------- *)
 
+  (* Utility lemmas *)
   Lemma vir_call_ev_nil i_t i_s t dv args :
     frame_inv i_t i_s -∗
     dval_rel dv dv -∗
@@ -103,23 +139,26 @@ Section mcfg_contextual.
 
 (* -------------------------------------------------------------------------- *)
 
-  Local Definition interp_mrec_ind :=
+  (* Induction hypothesis for [Proper_mrec] *)
+  Local Definition mrec_ind :=
     (λ Φ e_t e_s,
       ∀ (f g : ∀ T : Type, LLVMEvents.CallE T → L0'expr T) t dv args attr σ_t σ_s,
         ⌜e_t = observe (⟦ ⟅ f uvalue (Call t dv args attr) ⟆ ⟧ σ_t) ⌝ -∗
         ⌜e_s = observe (⟦ ⟅ g uvalue (Call t dv args attr) ⟆ ⟧ σ_s) ⌝ -∗
-        context_rel f g -∗
-        sim_indF interp_mrec_rec Φ
-        (observe (⟦ interp_mrec f (f uvalue (Call t dv args attr)) ⟧ σ_t))
-        (observe (⟦ interp_mrec g (g uvalue (Call t dv args attr)) ⟧ σ_s)))%I.
+        args_rel args args -∗
+        □ contains_base Φ -∗
+        □ context_rel f g -∗
+        sim_indF mrec_rec Φ
+        (observe (⟦ mrec f (Call t dv args attr) ⟧ σ_t))
+        (observe (⟦ mrec g (Call t dv args attr) ⟧ σ_s)))%I.
 
-  Local Instance interp_mrec_ind_ne:
-    NonExpansive (interp_mrec_ind: st_expr_rel' _ _ -d> st_expr_rel' _ _).
+  Local Instance mrec_ind_ne:
+    NonExpansive (mrec_ind: st_expr_rel' _ _ -d> st_expr_rel' _ _).
   Proof.
     solve_proper_prepare. clear -H. repeat f_equiv.
   Admitted.
 
-  Lemma Proper_mrec_interp_mrec_pred
+  Lemma Proper_mrec_pred
     (f g : ∀ T : Type, LLVMEvents.CallE T → L0'expr T) i_t i_s t dv args σ_t σ_s:
       (* Function address value and arguments are self-related *)
       dval_rel dv dv -∗
@@ -127,13 +166,13 @@ Section mcfg_contextual.
       (* Frame invariant holds *)
       frame_inv i_t i_s -∗
       (* Contexts are related *)
-      context_rel f g -∗
+      □ context_rel f g -∗
       state_interp σ_t σ_s ==∗
-      interp_mrec_pred (lift_rel ((λ _ _ : uvalue, frame_inv i_t i_s) ⤉))
-        (observe (⟦ interp_mrec f (f uvalue (Call t dv args [])) ⟧ σ_t))
-        (observe (⟦ interp_mrec g (g uvalue (Call t dv args [])) ⟧ σ_s)).
+      mrec_pred (lift_rel ((λ _ _ : uvalue, frame_inv i_t i_s) ⤉))
+        (observe (⟦ mrec f (Call t dv args []) ⟧ σ_t))
+        (observe (⟦ mrec g (Call t dv args []) ⟧ σ_s)).
   Proof.
-    rewrite /interp_mrec_pred.
+    rewrite /mrec_pred.
     iIntros "#Hdv #Hargs Hinv #Hrel SI".
     iExists f, g, t, dv, args, nil, σ_t, σ_s.
     do 2 (iSplitL ""; first done); iFrame "Hrel".
@@ -142,6 +181,25 @@ Section mcfg_contextual.
     iPoseProof (frame_inv_frame_WF with "Hinv") as "%Hframe_WF".
     iPoseProof (vir_call_ev_nil with "Hinv Hdv Hargs") as "Hev".
     iSpecialize ("Hrel" with "Hev SI").
+    iFrame "Hdv Hargs".
+
+    (* Base postcondition *)
+    iSplitL "".
+    { do 2 iModIntro. iIntros (??). iSplitL ""; iIntros "H".
+      - iDestruct "H" as "(H & Hr)"; done.
+      - iDestruct "H" as (????) "(SI&H)". (* TODO fact about [base] *)
+        iDestruct "H" as (??????) "H".
+        iFrame. iSplit.
+        { rewrite /base. subst.
+          iExists (σ_t0, v_t), (σ_s0, v_s). iPureIntro; split.
+          { apply EqAxiom.bisimulation_is_eq.
+            rewrite H4. by rewrite -itree_eta. }
+          { apply EqAxiom.bisimulation_is_eq.
+            rewrite H5. by rewrite -itree_eta. } }
+        subst.
+        iExists σ_t0, σ_s0, e_t, e_s; iFrame.
+        do 2 (iSplitL ""; [ done | ]).
+        iExists v_t, v_s; done. }
     iMod "Hrel".
 
     (* Establish postcondition. *)
@@ -149,7 +207,7 @@ Section mcfg_contextual.
     iIntros (??) "Hrel". rewrite /lift_rel.
     iDestruct "Hrel" as (????) "(SI & %Ht & %Hs & Hrel)"; subst.
     (* Access lifted postcondition *)
-    iDestruct "Hrel" as (????) "Hrel".
+    iDestruct "Hrel" as (????) "Hrel". rewrite /call_ans /=.
     simp vir_call_ans. iDestruct "Hrel" as "(?&?&?&#?)"; iFrame.
     (* Prove postcondition. *)
     iExists σ_t0, σ_s0, e_t0, e_s0; iFrame.
@@ -157,25 +215,32 @@ Section mcfg_contextual.
     iExists v_t, v_s; done.
   Qed.
 
-(* -------------------------------------------------------------------------- *)
+  (* Cases for [Proper_mrec] *)
+  Lemma Proper_mrec_base f g t dv args attr σ_t σ_s Ψ:
+    dval_rel dv dv -∗
+    args_rel args args -∗
+    <pers> contains_base Ψ -∗
+    <pers> context_rel f g -∗
+    Ψ (o⟦ ⟅ f uvalue (Call t dv args attr) ⟆ ⟧ σ_t)
+      (o⟦ ⟅ g uvalue (Call t dv args attr) ⟆ ⟧ σ_s) -∗
+    sim_mrec_ind Ψ
+      (o⟦ mrec f (Call t dv args attr) ⟧ σ_t)
+      (o⟦ mrec g (Call t dv args attr) ⟧ σ_s).
+  Proof.
+    iIntros "#Hdv #Hargs #Hbase #Hcrel HΨ".
+    iSpecialize ("Hbase" with "HΨ").
+    iDestruct "Hbase" as "(Hb & He)".
+    iDestruct "Hb" as (???) "%Hb".
 
-  (* ITree-related tactics *)
-  Ltac obs_hyp :=
-    match goal with
-      | [ H : {| _observe := observe _ |} = _ |- _] =>
-          let Hobs := fresh "Hobs" in
-          inversion H as [ Hobs ]; clear H
-    end.
+    do 2 simpobs_eqit.
+    apply interp_L2_conv_ret_inv in Hobs, Hobs0.
+    to_eq in Hobs; to_eq in Hobs0; subst; cbn.
 
-  (* Turn an [observe] hypothesis to an ITree equivalence. *)
-  Ltac simpobs_eqit :=
-    obs_hyp;
-    match goal with
-    | [ H : observe _ = _ |- _] =>
-        symmetry in H; apply Eqit.simpobs in H
-    end.
-
-(* -------------------------------------------------------------------------- *)
+    (* force unfold mrec *)
+    with_strategy transparent [mrec] unfold mrec.
+    rewrite Hobs Hobs0. cbn.
+    by provide_case: BASE.
+  Qed.
 
   Theorem Proper_mrec f g i_t i_s t dv args:
     (* Function address value and arguments are self-related *)
@@ -184,52 +249,57 @@ Section mcfg_contextual.
     (* Frame invariant holds *)
     frame_inv i_t i_s -∗
     (* Contexts are related *)
-    context_rel f g -∗
+    <pers> context_rel f g -∗
     mrec f (Call t dv args nil) ⪯ mrec g (Call t dv args nil)
     [[ (fun x y => frame_inv i_t i_s) ⤉ ]].
   Proof.
-    rewrite /mrec.
     iIntros "#Hdv #Hargs Hinv #Hrel"; iIntros (??) "SI".
 
     (* Initialize coinductive hypothesis. *)
-    iApply (sim_coindF_strong_coind interp_mrec_pred); cycle 1.
-    { iApply (Proper_mrec_interp_mrec_pred with "Hdv Hargs Hinv Hrel SI"). }
+    iApply (sim_coindF_strong_coind mrec_pred); cycle 1.
+    { iApply (Proper_mrec_pred with "Hdv Hargs Hinv Hrel SI"). }
 
     (* Set up context *)
-    iModIntro. iClear "Hdv Hrel". clear.
+    iModIntro. iClear "Hdv Hargs Hrel". clear.
     iIntros (Φ e_t e_s) "IH";
-    iDestruct "IH" as (??????????) "(#Hcrel & IH)"; subst.
+    iDestruct "IH" as (??????????) "(#Hdv & #Hargs & #Hbase & #Hcrel & IH)";
+      subst.
 
     (* Induction on simulation between (f call) and (g call). *)
     rewrite sim_coindF_unfold.
     iAssert (∀ Ψ e_t e_s, (sim_indF sim_coindF Ψ e_t e_s) -∗
-      interp_mrec_ind Ψ e_t e_s)%I as "Hgen"; last first.
+      mrec_ind Ψ e_t e_s)%I as "Hgen"; last first.
     { iSpecialize ("Hgen" with "IH").
-      iApply ("Hgen" $! _ _ _ _ _ _ _ _ eq_refl eq_refl with "Hcrel"). }
+      rewrite /mrec_ind.
+      iApply ("Hgen" $! _ _ _ _ _ _ _ _ eq_refl eq_refl with "Hargs Hbase Hcrel"). }
 
     (* Set up context *)
-    iClear "Hcrel". clear. iIntros (Ψ e_t e_s) "Hsim".
+    iClear "Hargs Hdv Hcrel Hbase"; clear.
+    iIntros (Ψ e_t e_s) "Hsim".
     iApply (sim_indF_strong_ind with "[] Hsim"); clear.
     iModIntro; iIntros (Ψ e_t e_s) "Hinner".
-    iIntros (??????????) "#Hcrel"; subst.
+    iIntros (??????????) "#Hargs #Hbase #Hcrel"; subst.
 
     (* [Hinner] for the "inner" expression, i.e. [e_s] *)
     rewrite /sim_expr_inner;
     cbn -[F] in *; rewrite sim_indF_unfold /sim_expr_inner.
-    iMod "Hinner"; to_inner interp_mrec_rec.
+    iMod "Hinner"; to_inner mrec_rec.
 
     (* Case analysis on the inductive information. *)
-    iDestruct "Hinner" as ( c ) "Hinner";
-      destruct c; try case_solve; try done.
+    iDestruct "Hinner" as ( c ) "Hinner"; destruct c; try case_solve; try done.
 
     (* [BASE] case *)
-    { admit. }
+    { iApply (Proper_mrec_base with "Hargs Hbase Hcrel Hinner"). }
+
     (* [STUTTER_L] case *)
     { admit. }
+
     (* [STUTTER_R] case *)
     { admit. }
+
     (* [TAU_STEP] case *)
     { admit. }
+
     (* [VIS] case *)
     { admit. }
 
@@ -238,11 +308,6 @@ Section mcfg_contextual.
 
     (* [EXC] case *)
     { simpobs_eqit; by eapply interp_L2_conv_failure_inv in Hobs. }
-
-
-
-
-
   Admitted. (* TODO : Port over proof *)
 
 (* -------------------------------------------------------------------------- *)
